Introduce DynaArrayList with dynamic insert operation

caseStudy/ADT/List/Impl/DynaArrayList.dfy
@@ -1,20 +1,20 @@
 include "../../../../theory/math/ExpReal.dfy"
 include "../../../../theory/math/TypeR0.dfy"
 include "../../../../theory/ComplexityR0.dfy"
-include "../List.dfy"
-include "./LemArrayList.dfy"
+include "../DynaList.dfy"
+include "./LemDynaArrayList.dfy"
 
 /******************************************************************************
-  Array implementation of a List
+  Dynamic Array implementation of a List
 ******************************************************************************/
 
-module ArrayList refines List {
+module DynaArrayList refines DynaList {
 
   import opened ExpReal
   import opened ComplexityR0
-  import opened LemArrayList
+  import opened LemDynaArrayList
 
-  class ArrayList<T(0)> extends List<T> {
+  class DynaArrayList<T(0)> extends DynaList<T> {
 
     var arr:array<T>
     var nElems:nat
@@ -87,20 +87,55 @@ module ArrayList refines List {
       requires Valid()
     {
       nElems == arr.Length
-    }    
+    }        
 
     /******************************************************************************
       Update operations
     ******************************************************************************/
 
+    // Increment array capacity by a multiplicative factor m > 1
+    method Grow(m:nat) returns (ghost t:R0) 
+      modifies this, Repr()
+      // Pre: 
+      requires Valid()
+      requires m > 1
+      // Post:
+      ensures Valid() && fresh(Repr() - old(Repr()))
+      ensures !IsFull()
+      ensures arr.Length == m*old(arr.Length) > old(arr.Length)
+      ensures arr[..nElems] == old(arr[..nElems])
+      // Complexity:
+      ensures  var N := old(arr.Length); && t == Tgrow(m,N,Size())
+                                         && t <= Tgrow(m,N,N)
+                                         && tIsBigO(N, t as R0, linGrowth())      
+    {   
+      var N := arr.Length;
+
+      // Allocate new array
+      var newArr := new T[m*N];
+      t := (m*N) as R0;
+      
+      // Copy old array content to new array
+      forall i | 0 <= i < Size() { 
+        newArr[i] := arr[i]; 
+      }
+      t := t + Size() as R0;
+
+      // Update current array
+      arr := newArr;
+      assert forall j :: 0 <= j < |elems| ==> arr[j] == elems[j];
+    
+      assert t == (m*N + Size()) as R0 == Tgrow(m,N,Size()) <= Tgrow(m,N,N);
+      assert (N => Tgrow(m,N,N)) in O(linGrowth()) by { var c, n0 := lem_Grow_TgrowBigOlin(m); }    
+    }
+
     // Inserts element x at position k in the list
     method Insert(k:nat, x:T) returns (ghost t:R0)
       modifies this, Repr()    
-      // Pre:
+      // Pre:      
       requires Valid()
       requires 0 <= k <= Size()
-      requires !IsFull()
-      // Post:
+      // Post:      
       ensures  Valid() && fresh(Repr() - old(Repr()))
       ensures  Size() == old(Size()) + 1
       ensures  forall j :: 0 <= j < k           ==> Get(j).0 == old(Get(j).0)    // [0, k)           is unchanged  
@@ -114,18 +149,29 @@ module ArrayList refines List {
       var N := Size();
       t := 0.0;
 
+      // Double array size if neccesary
+      if IsFull() { 
+        assert nElems == N == arr.Length;
+        t := Grow(2); 
+        assert t == Tgrow(2,N,N) == (3*N) as R0; 
+      }
+      assert !IsFull();
+      assert N < arr.Length;
+      assert t <= (3*N) as R0; 
+      assert arr[..N] == elems;
+
       // Update model
       elems := elems[..k] + [x] + elems[k..];
-      
+
       // Update array:
-      // 1. Shift (k, n] to the right
+      // 1. Shift (k, N] to the right
       var i := N;
       while i > k
         modifies arr
-        invariant k <= i <= N < arr.Length
+        invariant k <= i <= N < arr.Length    
         invariant arr[..i]      == old(arr[..i])   // [0, i) is unchanged  
-        invariant arr[i+1..N+1] == old(arr[i..N])  // (i, N] is right shifted        
-        invariant t == (N - i) as R0
+        invariant arr[i+1..N+1] == old(arr[i..N])  // (i, N] is right shifted      
+        invariant t <= (3*N + N - i) as R0
         decreases i
       {
         arr[i] := arr[i-1]; // shift right
@@ -139,13 +185,13 @@ module ArrayList refines List {
       assert i == k;
       arr[k] := x;
       assert arr[..k] == old(arr[..k]);  // [0, k) is unchanged
-
+    
       // Update number of elements
       nElems := nElems + 1;
 
-      assert t == (N - k) as R0 == Tinsert(N, k) 
-               <= N as R0       == Tinsert2(N);
-      assert Tinsert2 in O(linGrowth()) by { var c, n0 := lem_Insert_Tinsert2BigOlin(); }      
+      assert t <= (4*N - k) as R0 == Tinsert(N, k)
+               <= (4*N) as R0     == Tinsert2(N);
+      assert Tinsert2 in O(linGrowth()) by { var c, n0 := lem_Insert_Tinsert2BigOlin(k); }            
     }
 
     // Deletes element at position k in the list
