caseStudy/ADT/List/Impl/LemDynaArrayList.dfy
@@ -3,10 +3,10 @@ include "../../../../theory/math/TypeR0.dfy"
 include "../../../../theory/ComplexityR0.dfy"
 
 /******************************************************************************
-  Auxiliary module for ArrayList verification
+  Auxiliary module for DynaArrayList verification
 ******************************************************************************/
 
-module LemArrayList {
+module LemDynaArrayList {
 
   import opened ExpReal
   import opened TypeR0
@@ -36,29 +36,56 @@ module LemArrayList {
     assert bigOfrom(c, n0, Tget, constGrowth());
   }
 
+  // Complexity analysis for Grow operation 
+
+
+  ghost function Tgrow(m:nat, N:nat, n:nat) : R0
+  {
+    (m*N + n) as R0
+  }
+
+  lemma lem_Grow_TgrowBigOlin(m:nat) returns (c:R0, n0:nat) 
+    ensures bigOfrom(c, n0, (N => Tgrow(m,N,N)), linGrowth())
+  {
+      c, n0 := (m+1) as R0, 1;
+      forall n:nat | 0 <= n0 <= n
+        ensures (N => Tgrow(m,N,N))(n) <= c*linGrowth()(n)
+      {
+        calc {
+             (N => Tgrow(m,N,N))(n);
+          == (m*n + n) as R0;
+          == ((m+1)*n) as R0;
+          == { lem_expOne(n as R0); }
+            c*exp(n as R0, 1.0);
+          == c*linGrowth()(n);   
+        }
+      }
+      assert bigOfrom(c, n0, (N => Tgrow(m,N,N)), linGrowth());
+  }
+
   // Complexity analysis for Insert operation 
 
   ghost function Tinsert(N:nat, k:nat) : R0
     requires N >= k
   {
-    (N - k) as R0
+    (4*N - k) as R0
   }
 
   ghost function Tinsert2(N:nat) : R0
   {
-    N as R0
+    (4*N) as R0
   }  
 
-  lemma lem_Insert_Tinsert2BigOlin() returns (c:R0, n0:nat) 
+  lemma lem_Insert_Tinsert2BigOlin(k:nat) returns (c:R0, n0:nat) 
     ensures bigOfrom(c, n0, Tinsert2, linGrowth())
   {
-    c, n0 := 1.0, 1;
+    c, n0 := 4.0, 1;
     forall n:nat | 0 <= n0 <= n
       ensures Tinsert2(n) <= c*linGrowth()(n)
     {
       calc {
            Tinsert2(n);
-        == n as R0;
+        == (4*n) as R0;
         <= c*n as R0;
         == { lem_expOne(n as R0); }
            c*exp(n as R0, 1.0);
