caseStudy/ADT/List/List.dfy
@@ -18,7 +18,7 @@ module List {
     ******************************************************************************/
 
     // Returns true iff the list is full
-    predicate Full()
+    predicate IsFull()
       reads this, Repr()
       // Pre:
       requires Valid() 
@@ -33,12 +33,12 @@ module List {
       // Pre:
       requires Valid()
       requires 0 <= k <= Size()
-      requires !Full()
+      requires !IsFull()
       // Post:
       ensures  Valid()
       ensures  Size() == old(Size()) + 1
-      ensures  forall j :: 0 <= j < k           ==> Get(j).0 == old(Get(j).0)    // [0, k) is unchanged  
-      ensures  forall j :: k < j <= old(Size()) ==> Get(j).0 == old(Get(j-1).0)  // (k, n] is right shifted  
+      ensures  forall j :: 0 <= j < k           ==> Get(j).0 == old(Get(j).0)    // [0, k)           is unchanged  
+      ensures  forall j :: k < j <= old(Size()) ==> Get(j).0 == old(Get(j-1).0)  // (k, old(Size())] is right shifted  
       ensures  Get(k).0 == x                                                     // xs[k] == x
 
     // Deletes element at position k in the list
